sledge/semantics/miscScript.sml
@@ -9,7 +9,7 @@
  * could be upstreamed to HOL, and should eventually. *)
 
 open HolKernel boolLib bossLib Parse;
-open listTheory rich_listTheory arithmeticTheory integerTheory;
+open listTheory rich_listTheory arithmeticTheory integerTheory llistTheory pathTheory;
 open integer_wordTheory wordsTheory;
 open finite_mapTheory open logrootTheory numposrepTheory;
 open settingsTheory;
@@ -163,7 +163,7 @@ Proof
 QED
 
 Theorem mod_n2l:
-  ∀d n. 0 < d ⇒ map (\x. x MOD d) (n2l d n) = n2l d n
+  ∀d n. 0 < d ⇒ map (λx. x MOD d) (n2l d n) = n2l d n
 Proof
   rw [] >> drule n2l_BOUND >> disch_then (qspec_then `n` mp_tac) >>
   qspec_tac (`n2l d n`, `l`) >>
@@ -192,7 +192,7 @@ Proof
     conj_tac
     >- (
       simp [int_mod, INT_ADD_ASSOC,
-            intLib.COOPER_PROVE ``!x y (z:int). x - (y + z - a) = x - y - z + a``] >>
+            intLib.COOPER_PROVE ``∀x y (z:int). x - (y + z - a) = x - y - z + a``] >>
       qexists_tac `-((i + s1) / s2)` >>
       intLib.COOPER_TAC) >>
     `&INT_MIN (:α) = s1` by (unabbrev_all_tac >> rw [INT_MIN_def]) >>
@@ -228,7 +228,7 @@ Proof
       fs [Abbr `s2`] >>
       `s1 = &INT_MIN (:'a)` by intLib.COOPER_TAC >> rw [] >>
       irule INT_LESS_MOD >> rw [] >>
-      fs [intLib.COOPER_PROVE ``!(x:int) y. ¬(x ≤ y) ⇔ y < x``] >> rw [] >>
+      fs [intLib.COOPER_PROVE ``∀(x:int) y. ¬(x ≤ y) ⇔ y < x``] >> rw [] >>
       full_simp_tac std_ss [GSYM INT_MUL] >>
       qpat_abbrev_tac `s = &INT_MIN (:α)`
       >- (
@@ -239,6 +239,347 @@ Proof
         intLib.COOPER_TAC)
       >- intLib.COOPER_TAC) >>
     simp [INT_MOD_PLUS])
+QED
+
+(* ----- Theorems about lazy lists ----- *)
+
+Theorem toList_some:
+  ∀ll l. toList ll = Some l ⇔ ll = fromList l
+Proof
+  Induct_on `l` >> rw [] >>
+  Cases_on `ll` >> rw [toList_THM] >>
+  metis_tac []
+QED
+
+
+(* ----- Theorems about labelled transition system paths ----- *)
+
+Theorem take_all:
+  ∀p n. length p = Some n ⇒ take (n - 1) p = p
+Proof
+  Induct_on `n` >> rw []
+  >- metis_tac [length_never_zero] >>
+  qspec_then `p` mp_tac path_cases >> rw [] >> fs [alt_length_thm] >>
+  first_x_assum drule >> rw [] >>
+  Cases_on `n` >> fs [length_never_zero]
+QED
+
+Theorem el_plink:
+  ∀n p1 p2.
+    n ∈ PL (plink p1 p2) ∧ last p1 = first p2 ⇒
+    el n (plink p1 p2) = (if n ∈ PL p1 then el n p1 else el (Suc n - THE (length p1)) p2)
+Proof
+  Induct_on `n` >> rw [first_plink] >>
+  qspec_then `p1` mp_tac path_cases >> rw [] >> fs [] >>
+  rw [alt_length_thm] >>
+  first_x_assum drule >> rw [] >>
+  Cases_on `length q` >> fs [PL_def, length_def]
+QED
+
+Theorem el_pcons:
+  ∀n x l p. el n (pcons x l p) = if n = 0 then x else el (n - 1) p
+Proof
+  Induct_on `n` >>
+  rw []
+QED
+
+Theorem first_pconcat[simp]:
+  ∀p1 l p2. first (pconcat p1 l p2) = first p1
+Proof
+  rw [] >> qspec_then `p1` mp_tac path_cases >> rw [] >> rw [pconcat_thm]
+QED
+
+Theorem el_pconcat:
+  ∀n p1 l p2.
+    n ∈ PL (pconcat p1 l p2) ⇒
+    el n (pconcat p1 l p2) = (if n ∈ PL p1 then el n p1 else el (n - THE (length p1)) p2)
+Proof
+  Induct_on `n` >> rw [] >>
+  qspec_then `p1` mp_tac path_cases >> rw [] >> fs [pconcat_thm] >>
+  rw [alt_length_thm] >>
+  first_x_assum drule >> rw [] >>
+  Cases_on `length q` >> fs [PL_def, length_def]
+QED
+
+Theorem labels_pconcat[simp]:
+  ∀p1 l p2. labels (pconcat p1 l p2) = LAPPEND (labels p1) (l:::labels p2)
+Proof
+  rw [pconcat_def, labels_LMAP, path_rep_bijections_thm, LMAP_APPEND]
+QED
+
+Theorem length_pconcat:
+  ∀p1 l p2 l1 l2.
+    length p1 = Some l1 ∧ length p2 = Some l2
+    ⇒
+    length (pconcat p1 l p2) = Some (l1 + l2)
+Proof
+  rw [pconcat_def, length_def, path_rep_bijections_thm, finite_def,
+      LFINITE_APPEND] >>
+  rw [] >>
+  `LFINITE (LAPPEND (snd (fromPath p1)) ((l,first p2):::snd (fromPath p2)))`
+  by rw [LFINITE_APPEND] >>
+  imp_res_tac LFINITE_toList >> rw [] >>
+  imp_res_tac toList_LAPPEND_APPEND >> fs [toList_THM]
+QED
+
+Theorem take_pconcat:
+  ∀n p1 l p2.
+    take n (pconcat p1 l p2) =
+      if n ∈ PL p1 then
+        take n p1
+      else
+        pconcat p1 l (take (n - THE (length p1)) p2)
+Proof
+  Induct_on `n` >> rw []
+  >- (
+    fs [PL_def] >>
+    qspec_then `p1` mp_tac path_cases >> rw [] >> rw [pconcat_thm] >>
+    fs [finite_def, alt_length_thm])
+  >- (
+    qspec_then `p1` mp_tac path_cases >> rw [] >> rw [pconcat_thm] >>
+    fs [PL_def])
+  >- (
+    qspec_then `p1` mp_tac path_cases >> rw [] >> rw [pconcat_thm] >>
+    fs [PL_def, alt_length_thm, finite_length])
+QED
+
+Theorem last_pconcat[simp]:
+  ∀p1. finite p1 ⇒ ∀l p2. last (pconcat p1 l p2) = last p2
+Proof
+  ho_match_mp_tac finite_path_ind >>
+  rw [pconcat_thm]
+QED
+
+Theorem length_labels:
+  ∀p n. length p = Some (Suc n) ⇔ LLENGTH (labels p) = Some n
+Proof
+  Induct_on `n` >> rw [] >>
+  qspec_then `p` mp_tac path_cases >> rw [] >> rw [alt_length_thm, length_never_zero]
+QED
+
+Theorem ltake_fromList2:
+  ∀n l. n ≤ length l ⇒ LTAKE n (fromList l) = Some (take n l)
+Proof
+  Induct_on `l` >> rw [] >>
+  Cases_on `n` >> fs []
+QED
+
+Theorem el_take:
+  ∀p m n. n ∈ PL p ∧ m ≤ n ⇒ el m (take n p) = el m p
+Proof
+  Induct_on `n` >> rw [] >> rw [el_pcons] >>
+  first_x_assum (qspecl_then [`tail p`, `m-1`] mp_tac) >>
+  impl_tac
+  >- (
+    fs [PL_def] >> rw [] >>
+    qspec_then `p` mp_tac path_cases >> rw [] >> fs [alt_length_thm] >>
+    fs [finite_length] >> fs []) >>
+  rw [] >>
+  Cases_on `m` >> rw []
+QED
+
+Theorem nth_label_pcons:
+  (∀n s l p. nth_label 0 (pcons s l p) = l) ∧
+  (∀n s l p. nth_label (Suc n) (pcons s l p) = nth_label n p)
+Proof
+  rw []
+QED
+
+Theorem okpath_pointwise_imp1:
+  ∀p. (∀n. Suc n ∈ PL p ⇒ r (el n p) (nth_label n p) (el (Suc n) p)) ⇒ okpath r p
+Proof
+  ho_match_mp_tac okpath_co_ind >> rw [] >>
+  qspec_then `p` mp_tac path_cases >> rw [] >> rw [first_thm] >>
+  fs [PL_def]
+  >- (first_x_assum (qspec_then `0` mp_tac) >> rw []) >>
+  rw [el_pcons]
+  >- (first_x_assum (qspec_then `1` mp_tac) >> rw [] >> fs [el_pcons, nth_label_compute])
+  >- (
+    first_x_assum (qspec_then `Suc n` mp_tac) >> rw [] >>
+    Cases_on `n` >> fs [])
+QED
+
+Theorem okpath_pointwise_imp2:
+  ∀p. okpath r p ∧ finite p ⇒ (∀n. Suc n ∈ PL p ⇒ r (el n p) (nth_label n p) (el (Suc n) p))
+Proof
+  ho_match_mp_tac finite_okpath_ind >> rw [] >>
+  Cases_on `n` >> fs []
+QED
+
+Theorem okpath_pointwise:
+  ∀r p. okpath r p ⇔ (∀n. Suc n ∈ PL p ⇒ r (el n p) (nth_label n p) (el (Suc n) p))
+Proof
+  rw [] >> eq_tac >> rw [okpath_pointwise_imp1] >>
+  `okpath r (take (Suc n) p)` by metis_tac [okpath_take] >>
+  `finite (take (Suc n) p)` by metis_tac [finite_take] >>
+  drule okpath_pointwise_imp2 >> simp [] >>
+  disch_then (qspec_then `n` mp_tac) >> simp [el_pcons] >>
+  Cases_on `n = 0` >> simp [] >>
+  `n ∈ PL (tail p)`
+  by (
+    fs [PL_def] >>
+    qspec_then `p` mp_tac path_cases >> rw [] >> rw [first_thm] >>
+    fs [alt_length_thm] >> fs [finite_length] >> fs []) >>
+  simp [el_take] >>
+  `el (n - 1) (tail p) = el n p` by (Cases_on `n` >> rw []) >>
+  simp [] >>
+  `∃m. n = Suc m` by intLib.COOPER_TAC >>
+  `Suc m ∈ PL (tail p)` by fs [PL_def] >>
+  ASM_REWRITE_TAC [nth_label_pcons] >>
+  simp [nth_label_take]
+QED
+
+Theorem length_plink:
+  ∀p1 p2 l1 l2.
+    length p1 = Some l1 ∧ length p2 = Some l2
+    ⇒
+    length (plink p1 p2) = Some (l1 + l2 - 1)
+Proof
+  Induct_on `l1` >> rw [] >> fs [length_never_zero] >>
+  qspec_then `p1` mp_tac path_cases >> rw [plink_def] >>
+  fs [alt_length_thm] >> res_tac >> fs [ADD1] >>
+  `l1 ≠ 0` by metis_tac [length_never_zero] >>
+  decide_tac
+QED
+
+Theorem take_plink:
+  ∀n p1 p2.
+    take n (plink p1 p2) =
+      if Suc n ∈ PL p1 then
+        take n p1
+      else
+        plink p1 (take ((Suc n) - THE (length p1)) p2)
+Proof
+  Induct_on `n` >> rw []
+  >- (
+    fs [PL_def] >>
+    qspec_then `p1` mp_tac path_cases >> rw [] >>
+    fs [finite_def, alt_length_thm])
+  >- (
+    fs [PL_def] >>
+    qspec_then `p1` mp_tac path_cases >> rw []>> rw [plink_def] >>
+    fs [finite_length, alt_length_thm] >> rfs [] >>
+    Cases_on `n` >> fs [length_never_zero])
+  >- (
+    qspec_then `p1` mp_tac path_cases >> rw []>> rw [plink_def] >>
+    fs [PL_def])
+  >- (
+    qspec_then `p1` mp_tac path_cases >> rw []>> rw [plink_def] >>
+    fs [PL_def])
+  >- (
+    qspec_then `p1` mp_tac path_cases >> rw [] >> rw [] >>
+    fs [PL_def, alt_length_thm])
+  >- (
+    qspec_then `p1` mp_tac path_cases >> rw [] >> fs [alt_length_thm] >>
+    `finite q` by fs [PL_def] >>
+    fs [finite_length])
+QED
+
+Theorem unfold_last_lem:
+  ∀path. finite path ⇒
+    ∀proj f s. path = unfold proj f s ⇒
+    ∃y. proj y = last path ∧ f y = None ∧ (1 ∈ PL path ⇒ ∃x l. f x = Some (y, l))
+Proof
+  ho_match_mp_tac finite_path_ind >> rw []
+  >- (
+    fs [Once unfold_thm] >> Cases_on `f s` >> fs []
+    >- metis_tac [] >>
+    split_pair_case_tac >> fs []) >>
+  pop_assum mp_tac >> simp [Once unfold_thm] >> Cases_on `f s` >> simp [] >>
+  split_pair_case_tac >> rw [] >>
+  first_x_assum (qspecl_then [`proj`, `f`, `s'`] mp_tac) >> simp [] >>
+  Cases_on `1 ∈ PL (unfold proj f s')` >> rw [] >>
+  fs [PL_def] >>
+  fs [Once unfold_thm] >>
+  Cases_on `f s'` >> fs [alt_length_thm] >> rw [] >-
+  metis_tac [] >>
+  split_pair_case_tac >> fs [] >> rw [] >> fs [alt_length_thm, finite_length] >>
+  rfs [] >>
+   `n = 0 ∨ n = 1` by decide_tac >> fs [length_never_zero]
+QED
+
+Theorem unfold_last:
+  ∀proj f s.
+    finite (unfold proj f s)
+    ⇒
+    ∃y. proj y = last (unfold proj f s) ∧ f y = None ∧
+    (1 ∈ PL (unfold proj f s) ⇒ ∃x l. f x = Some (y, l))
+Proof
+  metis_tac [unfold_last_lem]
+QED
+
+Theorem pconcat_to_plink_finite:
+  ∀p1. finite p1 ⇒ ∀l p2. pconcat p1 l p2 = plink p1 (pcons (last p1) l p2)
+Proof
+  ho_match_mp_tac finite_path_ind >> rw [pconcat_thm]
+QED
+
+Definition opt_funpow_def:
+  (opt_funpow f 0 x = Some x) ∧
+  (opt_funpow f (Suc n) x = option_join (option_map f (opt_funpow f n x)))
+End
+
+Theorem opt_funpow_alt:
+  ∀n f s.
+    opt_funpow f (Suc n) s = option_join (option_map (opt_funpow f n) (f s))
+Proof
+  Induct_on `n` >> rw [] >> Cases_on `f s` >> rw [] >>
+  `1 = Suc 0` by decide_tac >>
+  ASM_REWRITE_TAC [] >>
+  rw [opt_funpow_def] >>
+  fs [opt_funpow_def]
+QED
+
+Theorem unfold_finite_funpow_lem:
+  ∀f proj s x.
+    opt_funpow (option_map fst ∘ f) m s = Some x ∧ f x = None
+    ⇒
+    finite (unfold proj f s)
+Proof
+  Induct_on `m` >> rw [opt_funpow_def] >>
+  simp [Once unfold_thm] >>
+  CASE_TAC >> fs [] >> split_pair_case_tac >> fs [] >> rw [] >>
+  Cases_on `opt_funpow (option_map fst ∘ f) m s` >> rw [] >>
+  fs [optionTheory.OPTION_MAP_DEF] >>
+  first_x_assum irule >> qexists_tac `x` >> rw [] >>
+  `opt_funpow (option_map fst ∘ f) (Suc m) s = Some (fst z)` by fs [opt_funpow_def] >>
+  rfs [opt_funpow_alt]
+QED
+
+Theorem unfold_finite_funpow:
+  ∀f proj s m.
+    opt_funpow (option_map fst ∘ f) m s = None
+    ⇒
+    finite (unfold proj f s)
+Proof
+  rw [] >> irule unfold_finite_funpow_lem >>
+  Induct_on `m` >> rw [] >> fs [opt_funpow_def] >>
+  Cases_on `opt_funpow (option_map fst ∘ f) m s` >> fs [] >>
+  metis_tac []
+QED
+
+Theorem unfold_finite:
+  ∀proj f s.
+    (∃R. WF R ∧ ∀n s2 l s3. opt_funpow (option_map fst o f) n s = Some s2 ∧ f s2 = Some (s3, l) ⇒ R s3 s2)
+    ⇒
+    finite (unfold proj f s)
+Proof
+  rw [] >> drule relationTheory.WF_INDUCTION_THM >>
+  disch_then (qspecl_then [`λx. ∀n. opt_funpow (option_map fst o f) n s = Some x ⇒
+                                    ∃m. opt_funpow (option_map fst o f) m x = None`,
+                           `s`] mp_tac) >>
+  simp [] >>
+  impl_tac
+  >- (
+    rw [] >>
+    first_x_assum drule >> Cases_on `f x` >> simp []
+    >- (qexists_tac `Suc n` >> simp [opt_funpow_alt]) >>
+    PairCases_on `x'` >> rw [] >>
+    first_x_assum drule >> rw [] >>
+    first_x_assum (qspec_then `Suc n` mp_tac) >> simp [opt_funpow_def] >>
+    rw [] >>
+    qexists_tac `Suc m` >> rw [opt_funpow_alt]) >>
+  metis_tac [unfold_finite_funpow, opt_funpow_def]
 QED
 
 export_theory ();
