sledge/semantics/llvm_liveScript.sml
@@ -1,0 +1,176 @@
+(*
+ * Copyright (c) Facebook, Inc. and its affiliates.
+ *
+ * This source code is licensed under the MIT license found in the
+ * LICENSE file in the root directory of this source tree.
+ *)
+
+(* Proofs about a shallowly embedded concept of live variables *)
+
+open HolKernel boolLib bossLib Parse;
+open pred_setTheory;
+open settingsTheory miscTheory llvmTheory llvm_propTheory;
+
+new_theory "llvm_live";
+
+numLib.prefer_num ();
+
+Definition inc_pc_def:
+  inc_pc ip = ip with i := ip.i + 1
+End
+
+(* The set of program counters the given instruction and starting point can
+ * immediately reach, withing a function *)
+Definition next_ips_def:
+  (next_ips (Ret _) ip = {}) ∧
+  (next_ips (Br _ l1 l2) ip =
+    { <| f := ip.f; b := Some l; i := 0 |> | l | l ∈ {l1; l2} }) ∧
+  (next_ips (Invoke _ _ _ _ l1 l2) ip =
+    { <| f := ip.f; b := Some l; i := 0 |> | l | l ∈ {l1; l2} }) ∧
+  (next_ips Unreachable ip = {}) ∧
+  (next_ips (Sub _ _ _ _ _ _) ip = { inc_pc ip }) ∧
+  (next_ips (Extractvalue _ _ _) ip = { inc_pc ip }) ∧
+  (next_ips (Insertvalue _ _ _ _) ip = { inc_pc ip }) ∧
+  (next_ips (Alloca _ _ _) ip = { inc_pc ip }) ∧
+  (next_ips (Load _ _ _) ip = { inc_pc ip }) ∧
+  (next_ips (Store _ _) ip = { inc_pc ip }) ∧
+  (next_ips (Gep _ _ _ _) ip = { inc_pc ip }) ∧
+  (next_ips (Ptrtoint _ _ _) ip = { inc_pc ip }) ∧
+  (next_ips (Inttoptr _ _ _) ip = { inc_pc ip }) ∧
+  (next_ips (Icmp _ _ _ _ _) ip = { inc_pc ip }) ∧
+  (next_ips (Call _ _ _ _) ip = { inc_pc ip }) ∧
+  (next_ips (Cxa_allocate_exn _ _) ip = { inc_pc ip }) ∧
+  (* TODO: revisit throw when dealing with exceptions *)
+  (next_ips (Cxa_throw _ _ _) ip = {  }) ∧
+  (next_ips (Cxa_begin_catch _ _) ip = { inc_pc ip }) ∧
+  (next_ips (Cxa_end_catch) ip = { inc_pc ip }) ∧
+  (next_ips (Cxa_get_exception_ptr _ _) ip = { inc_pc ip })
+End
+
+(* The path is a list of program counters that represent a statically feasible
+ * path through a function *)
+Inductive good_path:
+  (∀prog. good_path prog []) ∧
+
+  (∀ip i.
+    get_instr prog ip i
+    ⇒
+    good_path prog [ip]) ∧
+
+  (∀prog path ip1 i1 ip2.
+    get_instr prog ip1 i1 ∧
+    ip2 ∈ next_ips i1 ip1 ∧
+    good_path prog (ip2::path)
+    ⇒
+    good_path prog (ip1::ip2::path))
+End
+
+Definition arg_to_regs_def:
+  (arg_to_regs (Constant _) = {}) ∧
+  (arg_to_regs (Variable r) = {r})
+End
+
+(* The registers that an instruction uses *)
+Definition uses_def:
+  (uses (Ret (_, a)) = arg_to_regs a) ∧
+  (uses (Br a _ _) = arg_to_regs a) ∧
+  (uses (Invoke _ _ a targs _ _) =
+    arg_to_regs a ∪ BIGUNION (set (map (arg_to_regs o snd) targs))) ∧
+  (uses Unreachable = {}) ∧
+  (uses (Sub _ _ _ _ a1 a2) =
+    arg_to_regs a1 ∪ arg_to_regs a2) ∧
+  (uses (Extractvalue _ (_, a) _) = arg_to_regs a) ∧
+  (uses (Insertvalue _ (_, a1) (_, a2) _) =
+    arg_to_regs a1 ∪ arg_to_regs a2) ∧
+  (uses (Alloca _ _ (_, a)) = arg_to_regs a) ∧
+  (uses (Load _ _ (_, a)) = arg_to_regs a) ∧
+  (uses (Store (_, a1) (_, a2)) =
+    arg_to_regs a1 ∪ arg_to_regs a2) ∧
+  (uses (Gep _ _ (_, a) targs) =
+    arg_to_regs a ∪ BIGUNION (set (map (arg_to_regs o snd) targs))) ∧
+  (uses (Ptrtoint _ (_, a) _) = arg_to_regs a) ∧
+  (uses (Inttoptr _ (_, a) _) = arg_to_regs a) ∧
+  (uses (Icmp _ _ _ a1 a2) =
+    arg_to_regs a1 ∪ arg_to_regs a2) ∧
+  (uses (Call _ _ _ targs) =
+    BIGUNION (set (map (arg_to_regs o snd) targs))) ∧
+  (uses (Cxa_allocate_exn _ a) = arg_to_regs a) ∧
+  (uses (Cxa_throw a1 a2 a3) =
+    arg_to_regs a1 ∪ arg_to_regs a2 ∪ arg_to_regs a3) ∧
+  (uses (Cxa_begin_catch _ a) = arg_to_regs a) ∧
+  (uses (Cxa_end_catch) = {  }) ∧
+  (uses (Cxa_get_exception_ptr _ a) = arg_to_regs a)
+End
+
+(* The registers that an instruction assigns *)
+Definition assigns_def:
+  (assigns (Invoke r _ _ _ _ _) = {r}) ∧
+  (assigns (Sub r _ _ _ _ _) = {r}) ∧
+  (assigns (Extractvalue r _ _) = {r}) ∧
+  (assigns (Insertvalue r _ _ _) = {r}) ∧
+  (assigns (Alloca r _ _) = {r}) ∧
+  (assigns (Load r _ _) = {r}) ∧
+  (assigns (Gep r _ _ _) = {r}) ∧
+  (assigns (Ptrtoint r _ _) = {r}) ∧
+  (assigns (Inttoptr r _ _) = {r}) ∧
+  (assigns (Icmp r _ _ _ _) = {r}) ∧
+  (assigns (Call r _ _ _) = {r}) ∧
+  (assigns (Cxa_allocate_exn r _) = {r}) ∧
+  (assigns (Cxa_begin_catch r _) = {r}) ∧
+  (assigns (Cxa_get_exception_ptr r _) = {r}) ∧
+  (assigns _ = {})
+End
+
+Definition live_def:
+  live prog ip ⇔
+    { r | ∃path instr.
+            good_path prog (ip::path) ∧
+            get_instr prog (last (ip::path)) instr ∧
+            r ∈ uses instr ∧
+            ∀ip2 instr2. ip2 ∈ set (front (ip::path)) ∧ get_instr prog ip2 instr2 ⇒ r ∉ assigns instr2 }
+End
+
+Theorem get_instr_live:
+  ∀prog ip instr.
+    get_instr prog ip instr
+    ⇒
+    uses instr ⊆ live prog ip
+Proof
+  rw [live_def, SUBSET_DEF] >>
+  qexists_tac `[]` >> rw [Once good_path_cases] >>
+  qexists_tac `instr` >> simp [] >> metis_tac [IN_DEF]
+QED
+
+Triviality set_rw:
+  !s P. (!x. x ∈ s ⇔ P x) ⇔ s = P
+Proof
+  rw [] >> eq_tac >> rw [IN_DEF] >> metis_tac []
+QED
+
+Theorem live_gen_kill:
+  ∀prog ip instr ip'.
+    get_instr prog ip instr
+    ⇒
+    live prog ip = BIGUNION {live prog ip' | ip' ∈ next_ips instr ip} DIFF assigns instr ∪ uses instr
+Proof
+  rw [live_def, EXTENSION] >> eq_tac >> rw []
+  >- (
+    Cases_on `path` >> fs []
+    >- metis_tac [get_instr_func] >>
+    rename1 `ip::ip2::path` >>
+    qpat_x_assum `good_path _ _` mp_tac >> simp [Once good_path_cases] >> rw [] >>
+    Cases_on `x ∈ uses instr` >> fs [] >> simp [set_rw, PULL_EXISTS] >>
+    qexists_tac `ip2` >> qexists_tac `path` >> qexists_tac `instr'` >> rw [] >>
+    metis_tac [get_instr_func])
+  >- (
+    fs [] >>
+    qexists_tac `ip'::path` >> qexists_tac `instr'` >> rw []
+    >- (simp [Once good_path_cases] >> metis_tac []) >>
+    metis_tac [get_instr_func])
+  >- (
+    qexists_tac `[]` >> qexists_tac `instr` >> rw [] >>
+    simp [Once good_path_cases] >>
+    metis_tac [])
+QED
+
+export_theory ();
